

$$\vec{F} = -k \nabla T \quad \text{-- (1)}$$

$$\rho C_v \frac{dT}{dt} = -\nabla \cdot \vec{F}$$

$$C \frac{dT}{dt} = -\nabla \cdot \vec{F} \quad \text{-- (2)}$$

Derivating the eq. 1

$$\frac{d\vec{F}}{dt} = -k \nabla \frac{dT}{dt} - \nabla T \frac{dk}{dt} \quad \text{-- (3)}$$

Neglected

From 2 & 3

$$\frac{d\vec{F}}{dt} = -k \nabla \left[ \frac{-1}{C} \nabla \cdot \vec{F} \right]$$

$$\frac{d\vec{F}}{dt} = k \nabla \left[ \frac{1}{C} \nabla \cdot \vec{F} \right]$$

Multiplying both sides with test function 'v' and integrating over domain 'Ω'

$$\int_{\Omega} \frac{d\vec{F}}{dt} \vec{v} = \int_{\Omega} k \nabla \left[ \frac{1}{C} \nabla \cdot \vec{F} \right] \vec{v}$$

$$\int_{\Omega} \frac{1}{k} \frac{d\vec{F}}{dt} \vec{v} = \int_{\Omega} \nabla \left[ \frac{1}{C} \nabla \cdot \vec{F} \right] \vec{v}$$

$$\left( \frac{1}{k} \vec{u}, \vec{v} \right) \left( \frac{\vec{F}^{n+1} - \vec{F}^n}{dt} \right) = - \left( \frac{1}{C} \nabla \cdot \vec{u}, \nabla \cdot \vec{v} \right) \vec{F}^{n+1} \quad \text{Assuming zero boundary condition}$$

$$\left[ \left( \frac{1}{k} \vec{u}, \vec{v} \right) + \left( \frac{dt}{C} \nabla \cdot \vec{u}, \nabla \cdot \vec{v} \right) \right] \vec{F}^{n+1} = \left( \frac{1}{k} \vec{u}, \vec{v} \right) \vec{F}^n \quad -- (4)$$

$$\vec{F}^n = -k \nabla T^n$$

Multiplying both sides with test function 'v'  
and integrating over domain 'Ω'

$$\int_{\Omega} \frac{1}{k} \vec{F}^n \vec{v} = - \int_{\Omega} \nabla T^n \vec{v}$$

$$\left( \frac{1}{k} \vec{u}, \vec{v} \right) \vec{F}^n = - (\nabla u, \vec{v}) T^n$$

$$\vec{F}^n = - \left( \frac{1}{k} \vec{u}, \vec{v} \right)^{-1} (\nabla u, \vec{v}) T^n \quad -- (5)$$

From eqns 4 & 5

$$\left[ \left( \frac{1}{k} \vec{u}, \vec{v} \right) + \left( \frac{dt}{C} \nabla \cdot \vec{u}, \nabla \cdot \vec{v} \right) \right] \vec{F}^{n+1} = \left( \frac{1}{k} \vec{u}, \vec{v} \right) \left( - \left( \frac{1}{k} \vec{u}, \vec{v} \right)^{-1} (\nabla u, \vec{v}) T^n \right)$$

$$\left[ \left( \frac{1}{k} \vec{u}, \vec{v} \right) + \left( \frac{dt}{C} \nabla \cdot \vec{u}, \nabla \cdot \vec{v} \right) \right] \vec{F}^{n+1} = - (\nabla u, \vec{v}) T^n$$

Final  
equation

$$\vec{F}^{n+1} = - \left[ \left( \frac{1}{k} \vec{u}, \vec{v} \right) + \left( \frac{dt}{C} \nabla \cdot \vec{u}, \nabla \cdot \vec{v} \right) \right]^{-1} (\nabla u, \vec{v}) T^n$$

$$\left(\frac{1}{k} \vec{u}, \vec{v}\right) = \text{VectorFEMassIntegrator (InvTCond)}$$

$$(\nabla u, \vec{v}) = \text{WeakDiv} \rightarrow \text{MultTranspose}$$

$$\left(\frac{dt}{C} \nabla \cdot \vec{u}, \nabla \cdot \vec{v}\right) = \text{DivDivIntegrator}(dt * \text{InvTCap})$$